\documentclass[../notes.tex]{subfiles}

\pagestyle{main}
\renewcommand{\chaptermark}[1]{\markboth{\chaptername\ \thechapter\ (#1)}{}}
\setcounter{chapter}{27}

\begin{document}




\chapter{Rate Laws}
\section{Definitions and Methods of Determination}
\begin{itemize}
    \item \marginnote{4/8:}Consider a general chemical equation
    \begin{equation*}
        \ce{\nu_AA + \nu_BB -> \nu_YY + \nu_ZZ}
    \end{equation*}
    \item The extent of the reaction via the progress variable $\xi$ is
    \begin{align*}
        n_A(t) &= n_A(0)-\nu_A\xi(t)&
        n_Y(t) &= n_Y(0)+\nu_Y\xi(t)
    \end{align*}
    \item The rate of change (moles/second) is
    \begin{align*}
        \dv{n_A}{t} &= -\nu_A\dv{\xi}{t}&
        \dv{n_Y}{t} &= \nu_Y\dv{\xi}{t}
    \end{align*}
    \item Deriving the rate of reaction for a gas-based chemical reaction.
    \begin{itemize}
        \item Time-dependent concentration changes
        \begin{align*}
            \frac{1}{V}\dv{n_A}{t} &= \dv{[A]}{t} = -\frac{\nu_A}{V}\dv{\xi}{t}&
            \frac{1}{V}\dv{n_Y}{t} &= \dv{[Y]}{t} = -\frac{\nu_Y}{V}\dv{\xi}{t}
        \end{align*}
        \item The rate (or speed) of reaction, also known as the differential rate law, is
        \begin{equation*}
            v(t) = -\frac{1}{\nu_A}\dv{[A]}{t}
            = -\frac{1}{\nu_B}\dv{[B]}{t}
            = \frac{1}{\nu_Y}\dv{[Y]}{t}
            = \frac{1}{\nu_Z}\dv{[Z]}{t}
            = \frac{1}{V}\dv{\xi}{t}
        \end{equation*}
        \item All terms are positive.
        \item Rate laws with a constant $k$ are of the form
        \begin{equation*}
            v(t) = k[A]^{m_A}[B]^{m_B}
        \end{equation*}
        \item The exponents are known as \textbf{orders}.
        \item The overall order reaction is $\sum m_i$.
        \item The orders and overall order of the reaction depends on the fundamental reaction steps and the reaction mechanism.
    \end{itemize}
    \item For example, for the reaction \ce{2NO_{(g)} + O2_{(g)} -> 2NO2_{(g)}}, we have
    \begin{equation*}
        v(t) = -\frac{1}{2}\dv{[\ce{NO}]}{t}
        = -\dv{[\ce{O2}]}{t}
        = -\frac{1}{2}\dv{[\ce{NO2}]}{t}
    \end{equation*}
    \begin{itemize}
        \item It follows that $v(t)=k[\ce{NO}]^2[\ce{O2}]$.
        \item This is a rare elementary reaction that proceeds with the kinetics illustrated by the equation.
    \end{itemize}
    \item Rate laws must be determined by experiment.
    \begin{itemize}
        \item Multi-step reactions may have more complex rate law expressions.
        \item Oftentimes, $1/2$ exponents indicate more complicated mechanisms.
        \item For example, even an equation as simple looking as \ce{H2 + Br2 -> 2HBr} has rate law
        \begin{equation*}
            v(t) = \frac{k'[\ce{H2}][\ce{Br2}]^{1/2}}{1+k''[\ce{HBr}][\ce{Br2}]^{-1}}
        \end{equation*}
    \end{itemize}
    \item Determining rate laws.
    \begin{itemize}
        \item Method of isolation.
        \begin{itemize}
            \item Put in a large initial excess of $A$ so that it's concentration doesn't change that much; essentially incorporates $[A]^{m_A}$ into $k$ for determination of the order of $B$.
            \item We can then do the same thing the other way around.
        \end{itemize}
        \item Method of initial rates.
        \begin{itemize}
            \item We approximate
            \begin{equation*}
                v = -\frac{\dd{[A]}}{\nu_A\dd{t}}
                \approx -\frac{\Delta[A]}{\nu_A\Delta t}
                = k[A]^{m_A}[B]^{m_B}
            \end{equation*}
            \item Consider two different initial values of $[B]$, which we'll call $[B_1],[B_2]$. Then
            \begin{align*}
                v_1 &= -\frac{1}{\nu_A}\left( \frac{\Delta[A]}{\Delta t} \right)_1 = k[A]_0^{m_A}[B]_1^{m_B}&
                v_2 &= -\frac{1}{\nu_A}\left( \frac{\Delta[A]}{\Delta t} \right)_2 = k[A]_0^{m_A}[B]_2^{m_B}
            \end{align*}
            \item Take the logarithm and solve for $m_B$.
            \begin{equation*}
                m_B = \frac{\ln(v_1/v_2)}{\ln([B]_1/[B]_2)}
            \end{equation*}
        \end{itemize}
    \end{itemize}
    \item Does an example problem.
\end{itemize}



\section{Integrated Rate Laws}
\begin{itemize}
    \item \marginnote{4/11:}First order reactions have exponential integrated rate laws.
    \begin{itemize}
        \item Suppose \ce{A + B -> products}.
        \item Suppose the reaction is first order in \ce{A}.
        \item If the concentration of \ce{A} is $[\ce{A}]_0$ at $t=0$ and $[\ce{A}]$ at time $t$, then
        \begin{align*}
            v(t) = -\dv{[\ce{A}]}{t} &= k[\ce{A}]\\
            \int_{[\ce{A}]_0}^{[\ce{A}]}\frac{\dd{[\ce{A}]}}{[\ce{A}]} &= -\int_0^tk\dd{t}\\
            \ln\frac{[\ce{A}]}{[\ce{A}]_0} &= -kt\\
            [\ce{A}] &= [\ce{A}]_0\e[-kt]
        \end{align*}
        is the integrated rate law.
        \item Goes over both the concentration plot and the linear logarithmic plot.
    \end{itemize}
    \item The half-life of a first-order reaction is independent of the initial amount of reactant.
    \begin{itemize}
        \item The half-life is found from the point
        \begin{equation*}
            [\ce{A}(t_{1/2})] = \frac{[\ce{A}(0)]}{2}
            = \frac{[\ce{A}]_0}{2}
        \end{equation*}
        \item We have
        \begin{align*}
            \ln\frac{1}{2} &= -kt_{1/2}\\
            t_{1/2} &= \frac{\ln 2}{k} \approx \frac{0.693}{k}
        \end{align*}
        \item Notice that the above equation does not depend on $[\ce{A}]$ or $[\ce{B}]$!
    \end{itemize}
    \item Second order reactions have inverse concentration integrated rate laws.
    \begin{itemize}
        \item Suppose \ce{A + B -> products}, as before, and that the reaction is second order in \ce{A}.
        \item Then
        \begin{align*}
            -\dv{[\ce{A}]}{t} &= k[\ce{A}]^2\\
            \int_{[\ce{A}]_0}^{[\ce{A}]}-\frac{\dd{[\ce{A}]}}{[\ce{A}]^2} &= \int_0^tk\dd{t}\\
            \frac{1}{[\ce{A}]} &= \frac{1}{[\ce{A}]_0}+kt
        \end{align*}
        is the integrated rate law.
    \end{itemize}
    \item The half-life of a second-order reaction is dependent on the initial amount of reaction.
    \begin{itemize}
        \item We have that
        \begin{align*}
            \frac{1}{[\ce{A}]_0/2} &= \frac{1}{[\ce{A}]_0}+kt_{1/2}\\
            \frac{1}{[\ce{A}]_0} &= kt_{1/2}\\
            t_{1/2} &= \frac{1}{k[\ce{A}]_0}
        \end{align*}
    \end{itemize}
    \item If a reaction is $n^\text{th}$-order in a reactant for $n\geq 2$, then the integrated rate law is given by
    \begin{align*}
        -\dv{[\ce{A}]}{t} &= k[\ce{A}]^n\\
        \int_{[\ce{A}]_0}^{[\ce{A}]}-\frac{\dd{[\ce{A}]}}{[\ce{A}]^n} &= \int_0^tk\dd{t}\\
        \frac{1}{n-1}\left( \frac{1}{[\ce{A}]^{n-1}}-\frac{1}{[\ce{A}]_0^{n-1}} \right) &= kt
    \end{align*}
    \begin{itemize}
        \item The associated half life is
        \begin{align*}
            \frac{1}{n-1}\left( \frac{1}{([\ce{A}]_0/2)^{n-1}}-\frac{1}{[\ce{A}]_0^{n-1}} \right) &= kt_{1/2}\\
            \frac{1}{n-1}\cdot\frac{2^{n-1}-1}{[\ce{A}]_0^{n-1}} &= kt_{1/2}\\
            t_{1/2} &= \frac{2^{n-1}-1}{k(n-1)[\ce{A}]_0^{n-1}}
        \end{align*}
    \end{itemize}
    \item Second order reactions that are first order in each reactant.
    \begin{itemize}
        \item We have that
        \begin{align*}
            -\dv{[\ce{A}]}{t} = -\dv{[\ce{B}]}{t} &= k[\ce{A}][\ce{B}]\\
            kt &= \frac{1}{[\ce{A}]_0-[\ce{B}]_0}\ln\frac{[\ce{A}][\ce{B}]_0}{[\ce{B}][\ce{A}]_0}
        \end{align*}
        \item The actual determination is more complicated (there is a textbook problem that walks us through the derivation, though).
        \item When $[\ce{A}]_0=[\ce{B}]_0$, the integrated rate law simplifies to the second-order integrated rate laws in $[\ce{A}]$ and $[\ce{B}]$.
        \begin{itemize}
            \item In this limited case, the half-life is that of the second-order integrated rate law, too, i.e., $t_{1/2}=1/k[\ce{A}]_0$.
        \end{itemize}
    \end{itemize}
    \item The reaction paths and mechanism for parallel reactions.
    \begin{itemize}
        \item Suppose \ce{A} can become both \ce{B} and \ce{C} with respective rate constants $k_B$ and $k_C$.
        \item Then
        \begin{align*}
            \dv{[\ce{A}]}{t} &= -k_B[\ce{A}]-k_C[\ce{A}] = -(k_B+k_C)[\ce{A}]&
            \dv{[\ce{B}]}{t} &= k_B[\ce{A}]&
            \dv{[\ce{C}]}{t} &= k_C[\ce{A}]
        \end{align*}
        \item The integrated rate laws here are
        \begin{align*}
            [\ce{A}] &= [\ce{A}]_0\e[-(k_B+k_C)t]&
            [\ce{B}] &= \frac{k_B}{k_B+k_C}[\ce{A}]_0\left( 1-\e[-(k_B+k_C)t] \right)&
            [\ce{C}] &= \frac{k_C}{k_B+k_C}[\ce{A}]_0\left( 1-\e[-(k_B+k_C)t] \right)
        \end{align*}
        \item The ratio of product concentrations is
        \begin{equation*}
            \frac{[\ce{B}]}{[\ce{C}]} = \frac{k_B}{k_C}
        \end{equation*}
        \item The yield $\Phi_i$ is the probability that a given product $i$ will be formed from the decay of the reactant
        \begin{align*}
            \Phi_i &= \frac{k_i}{\sum_nk_n}&
            \sum_i\Phi_i &= 1
        \end{align*}
    \end{itemize}
    \item Example: If we have parallel reactions satisfying $k_B=2k_C$, then
    \begin{equation*}
        \Phi_C = \frac{k_C}{k_B+k_C}
        = \frac{k_C}{2k_C+k_C}
        = \frac{1}{3}
    \end{equation*}
\end{itemize}




\end{document}